More useful mach_sim definition

src/experiments/PEquiv.v
@@ -8,38 +8,75 @@ Require Import Arith List.
 
 Import ListNotations.
 
+(* A machine state is some subset of st_ty that is "well-formed" *)
 Record State :=
   { st_ty :> Type
   ; st_dec : forall (x y : st_ty), {x = y} + {x <> y}
   ; st_wf : st_ty -> Prop
   }.
 
+(* A machine is a transition system on well-formed states *)
 Record Mach (X:State) :=
   { m_step : X -> option X
   ; m_pres : forall x x', st_wf X x -> m_step x = Some x' -> st_wf X x'
   }.
 
-(* Homomorphic embedding *)
+(* A simulation relation between machines (partial fns on states)
+   preserving termination.
+
+   Note: we're not interested in the greatest such relation, defined
+   as the greatest fixpoint (vR. mach_sim_step M M' R):
+
+CoInductive mach_similarity {X:State} (M M':Mach X) : X -> X -> Prop :=
+mach_sim_fix : forall x x',
+  mach_sim_step M M' (mach_similarity M M') x x' ->
+  mach_similarity M M' x x'.
+
+   Instead, we define what it means for a relation R to be a
+   simulation w.r.t machines M and M' or, alternatively, the relation
+   on machines for a given simulation relation R. Note that when R is
+   an equivalence on states, this is just extensional functional
+   equivalence.
+
+   TODO: is it possible/desirable to augment mach_sim_step to indicate
+   that some states are unobservable? I.e. in addition to quotienting
+   states, can we introduce some flexibility w.r.t step size? This
+   would destroy the intuitivively appealing interpretation of
+   mach_sim as fn equivalence... *)
+
+Inductive mach_sim_step {X:State} (M M':Mach X) (R:X -> X -> Prop) : X -> X -> Prop :=
+| mach_sim_step_none : forall x x',
+  m_step M x = None ->
+  m_step M' x' = None ->
+  mach_sim_step M M' R x x'
+| mach_sim_step_one : forall x x' y y',
+  m_step M x = Some y ->
+  m_step M' x' = Some y' ->
+  R y y' ->
+  mach_sim_step M M' R x x'.
+
+Definition mach_sim {X:State} (R:X -> X -> Prop) (M M':Mach X) : Prop :=
+  forall x x', st_wf X x -> st_wf X x' ->
+  R x x' -> mach_sim_step M M' R x x'.
+
+
+
+
+(* Homomorphic embedding of machines (partial functions) *)
 Record HEmbed `(M:Mach X, N:Mach Y, U:X -> option Y) :=
-  { he_U_wf : forall x y, st_wf X x -> U x = Some y -> st_wf Y y
-  ; he_U_tot : forall x, st_wf X x -> exists y, U x = Some y
-  ; he_L : Y -> option X
+  { he_L : Y -> option X        (* loading *)
+
+  (* well-formedness and totality of load/unload *)
+  ; he_U_wf : forall x y, st_wf X x -> U x = Some y -> st_wf Y y
   ; he_L_wf : forall x y, st_wf Y y -> he_L y = Some x -> st_wf X x
+  ; he_U_tot : forall x, st_wf X x -> exists y, U x = Some y
   ; he_L_tot : forall y, st_wf Y y -> exists x, he_L y = Some x
+
+  (* definition of homomorphic embedding *)
   ; he_epi : forall y, st_wf Y y -> option_bind (he_L y) U = Some y
   ; he_spec : forall x, st_wf X x ->
     option_bind (m_step M x) U = option_bind (U x) (m_step N)
   }.
-
-(* Simulation between machines (partial fns on states) *)
-Definition mach_sim {X:State} (R:X -> X -> Prop) (M M':Mach X) : Prop :=
-  forall x x', st_wf X x -> st_wf X x' -> 
-    R x x' -> 
-    match m_step M x, m_step M' x' with
-    | Some y, Some y' => R y y'
-    | None, None => True
-    | _, _ => False
-    end.
 
 (* The main point is that when the "machine equivalence" diagram H
    between a machine M and a "more abstract" machine N, we have an
@@ -69,21 +106,23 @@ Lemma hembed_sim :
 Proof.
   unfold mach_sim. 
   intros ? ? Hwfx Hwfx' Heqxx'.
-  destruct (m_step M x) eqn:Hstep, (m_step hembed_mach x') eqn:Hstep';
-    unfold hembed_mach in *; simpl in *.
-  - rewrite <- Heqxx' in Hstep'.
+  destruct (m_step M x) as [x0|] eqn:Hstep, 
+           (m_step hembed_mach x') as [x0'|] eqn:Hstep';
+    unfold hembed_mach in Hstep'; simpl in Hstep'.
+  - eapply mach_sim_step_one; eauto.
+    rewrite <- Heqxx' in Hstep'.
     rewrite <- (he_spec H) in Hstep'; auto.
     rewrite Hstep in Hstep'. simpl in Hstep'.
-    destruct (U s) as [s'|] eqn:Heqs'; [|inversion Hstep'].
-    simpl in Hstep'. 
-    eapply f_equal with (f := fun x => option_bind x U) in Hstep'.
-    rewrite (he_epi H) in Hstep'. apply Hstep'.
+    destruct (U x0) as [y0 |] eqn:Heqs'; [|inversion Hstep'].
+    apply f_equal with (f:= fun x => option_bind x U) in Hstep'.
+    simpl in Hstep'. rewrite (he_epi H) in Hstep'. auto.
     apply (he_U_wf H) in Heqs'; auto.
     eapply (m_pres M) with (x:=x); eauto.
-  - rewrite <- Heqxx' in Hstep'.
+  - exfalso.
+    rewrite <- Heqxx' in Hstep'.
     rewrite <- (he_spec H) in Hstep'; auto.
     rewrite Hstep in Hstep'. simpl in Hstep'.
-    destruct (U s) as [s'|] eqn:Heqs'; [|inversion Hstep'].
+    destruct (U x0) as [y0|] eqn:Heqs'; [|inversion Hstep'].
     + simpl in Hstep'. 
       eapply f_equal with (f := fun x => option_bind x U) in Hstep'.
       simpl in *.
@@ -91,14 +130,11 @@ Proof.
       apply (he_U_wf H) in Heqs'; auto.
       eapply (m_pres M) with (x:=x); eauto.
     + apply m_pres, (he_U_tot H) in Hstep as [? ?]; auto. congruence.
-  - rewrite <- Heqxx' in Hstep'.
+  - exfalso.
+    rewrite <- Heqxx' in Hstep'.
     rewrite <- (he_spec H) in Hstep'; auto.
-    rewrite Hstep in Hstep'. simpl in Hstep'.
-    destruct (U s) as [s'|] eqn:Heqs'; [|inversion Hstep'].
-    + simpl in Hstep'. 
-      eapply f_equal with (f := fun x => option_bind x U) in Hstep'.
-      simpl in *. congruence.
-  - auto.
+    rewrite Hstep in Hstep'. simpl in Hstep'. congruence.
+  - eapply mach_sim_step_none; auto.
 Qed.
 
 End HEMBED_SIM.
